linear: prove has_type.subst

linear.v
@@ -228,57 +228,47 @@ Module expr.
 
 End expr.
 
-Fixpoint nth_set A (l : list A) (n : nat) (x : A) {struct n} : list A :=
-  match n with
-  | 0 =>
-    match l with
-    | [] => []
-    | y :: l => x :: l
-    end
-  | S n =>
-    match l with
-    | [] => []
-    | y :: l => y :: nth_set l n x
-    end
-  end.
 
-Lemma nth_set_length :
-  forall A n (l : list A) x,
-    length (nth_set l n x) = length l.
-Proof.
-  induction n; destruct l; simpl; intros x; auto.
-Qed.
 
-Lemma nth_error_nth_set :
-  forall A n2 n1 (l : list A) x,
-    n1 < List.length l ->
-    nth_error (nth_set l n1 x) n2 =
-    if Nat.eq_dec n1 n2 then Some x else nth_error l n2.
-Proof.
-  induction n2; destruct n1; destruct l; intros x LT; simpl in *;
-    try reflexivity;
-    try omega.
-  rewrite IHn2 by omega.
-  destruct Nat.eq_dec; auto.
-Qed.
-
-Fixpoint join (G1 G2 : list (option type.t)) : option (list (option type.t)) :=
-  match G1, G2 with
-  | [], [] => Some []
-  | g1 :: G1, g2 :: G2 =>
-    match g1, g2, join G1 G2 with
-    | Some ty, None, Some G => Some (Some ty :: G)
-    | None, Some ty, Some G => Some (Some ty :: G)
-    | None, None, Some G => Some (None :: G)
-    | _, _, _ => None
-    end
+Definition join_one (oty1 oty2 : option type.t) : option (option type.t) :=
+  match oty1, oty2 with
+  | None, None => Some None
+  | Some ty1, None => Some (Some ty1)
+  | None, Some ty2 => Some (Some ty2)
   | _, _ => None
   end.
+
+Lemma join_one_comm :
+  forall l1 l2,
+    join_one l1 l2 = join_one l2 l1.
+Proof.
+  unfold join_one.
+  intros.
+  repeat break_match; auto.
+Qed.
+
+Lemma join_one_assoc :
+  forall a1 a2 b,
+    match join_one a1 b with
+    | Some b' => join_one a2 b'
+    | None => None
+    end = match join_one a2 b with
+          | Some b' => join_one a1 b'
+          | None => None
+          end.
+Proof.
+  unfold join_one.
+  intros.
+  repeat break_match; congruence.
+Qed.
+
+Definition join G1 G2 := partial_zip.f join_one G1 G2.
+Hint Opaque join.
 
 Lemma join_nil :
   join [] [] = Some [].
 Proof.
-  reflexivity.
+  apply partial_zip.nil.
 Qed.
 Hint Resolve join_nil.
 
@@ -287,22 +277,25 @@ Lemma join_nil_inv :
     join G1 G2 = Some [] ->
     G1 = [] /\ G2 = [].
 Proof.
-  destruct G1, G2; simpl; try discriminate.
-  - intuition congruence.
-  - repeat break_match; discriminate.
+  apply partial_zip.nil_inv.
 Qed.
 
 Definition empty n : list (option type.t) := repeat None n.
+
+Lemma join_one_None_l :
+  forall oty,
+    join_one None oty = Some oty.
+Proof.
+  destruct oty; auto.
+Qed.
 
 Lemma join_empty_l :
   forall G,
     join (empty (length G)) G = Some G.
 Proof.
-  unfold empty.
-  induction G; simpl.
-  - reflexivity.
-  - rewrite IHG.
-    destruct a; reflexivity.
+  unfold join, empty.
+  intros G.
+  now rewrite partial_zip.id_l by auto using join_one_None_l.
 Qed.
 
 Lemma join_empty_l' :
@@ -313,6 +306,78 @@ Proof.
   intros.
   subst n.
   apply join_empty_l.
+Qed.
+
+Lemma join_length1 :
+  forall l1 l2 l3,
+    join l1 l2 = Some l3 ->
+    length l3 = length l1.
+Proof.
+  apply partial_zip.length1.
+Qed.
+
+Lemma join_length2 :
+  forall l1 l2 l3,
+    join l1 l2 = Some l3 ->
+    length l3 = length l2.
+Proof.
+  apply partial_zip.length2.
+Qed.
+
+Lemma join_unroll :
+  forall x1 x2 l1 l2,
+    join (x1 :: l1) (x2 :: l2) =
+    match join_one x1 x2 with
+    | None => None
+    | Some y =>
+      match join l1 l2 with
+      | None => None
+      | Some ys => Some (y :: ys)
+      end
+    end.
+Proof.
+  reflexivity.
+Qed.
+
+Lemma join_comm :
+  forall l1 l2,
+    join l1 l2 = join l2 l1.
+Proof.
+  apply partial_zip.comm.
+  apply join_one_comm.
+Qed.
+
+Lemma join_empty_r :
+  forall G,
+    join G (empty (length G)) = Some G.
+Proof.
+  intros.
+  now rewrite join_comm, join_empty_l.
+Qed.
+
+Lemma join_empty_r' :
+  forall G n,
+    length G = n ->
+    join G (empty n) = Some G.
+Proof.
+  intros.
+  subst.
+  now rewrite join_empty_r.
+Qed.
+
+Lemma join_assoc :
+  forall a1 a2 b,
+    match join a1 b with
+    | Some b' => join a2 b'
+    | None => None
+    end = match join a2 b with
+          | Some b' => join a1 b'
+          | None => None
+          end.
+Proof.
+  intros.
+  apply partial_zip.assoc.
+  apply join_one_assoc.
 Qed.
 
 Fixpoint is_empty (G : list (option type.t)) : Prop :=
@@ -331,39 +396,209 @@ Proof.
 Qed.
 Hint Resolve is_empty_empty.
 
-Fixpoint singleton (x : nat) (ty : type.t) (G : list (option type.t)) {struct G} : Prop :=
+Lemma is_empty_equal_empty :
+  forall l,
+    is_empty l ->
+    l = empty (length l).
+Proof.
+  induction l; cbn; intros IS.
+  - auto.
+  - destruct a; intuition.
+    f_equal. apply H.
+Qed.
+
+Fixpoint is_singleton (x : nat) (ty : type.t) (G : list (option type.t)) {struct G} : Prop :=
   match x, G with
   | 0, Some ty' :: G => ty = ty' /\ is_empty G
-  | S x, None :: G => singleton x ty G
+  | S x, None :: G => is_singleton x ty G
   | _, _ => False
   end.
 
-Lemma singleton_nth_error1 :
+Lemma is_singleton_nth_error1 :
   forall x ty G,
-    singleton x ty G ->
+    is_singleton x ty G ->
     List.nth_error G x = Some (Some ty).
-Admitted.
+Proof.
+  induction x; intros ty G IS; (destruct G; [|destruct o]); cbn in *; intuition.
+  congruence.
+Qed.
 
-Lemma singleton_nth_error2 :
-  forall x ty G,
-    singleton x ty G ->
-    forall y,
-      y < List.length G ->
-      x <> y ->
-      List.nth_error G y = Some None.
-Admitted.
+Definition big_join n Gs :=
+  partial_fold_left.f join (empty n) Gs.
+Hint Opaque big_join.
 
-Fixpoint big_join
-         (acc : list (option type.t))
-         (Gs : list (list (option type.t))) : option (list (option type.t)) :=
-  match Gs with
-  | [] => Some acc
-  | G1 :: Gs =>
-    match join acc G1 with
+Lemma big_join_unroll :
+  forall n G Gs,
+    big_join n (G :: Gs) =
+    match big_join n Gs with
+    | Some G' => join G G'
     | None => None
-    | Some G1' => big_join G1' Gs
-    end
-  end.
+    end.
+Proof.
+  unfold big_join.
+  intros n G Gs.
+  pose proof partial_fold_left.push_step join join_assoc as Push.
+  now rewrite <- Push.
+Qed.
+
+Lemma big_join_map_cons_None2 :
+  forall n Gs,
+    big_join (S (S n)) (map (fun x => None :: None :: x) Gs) =
+    match big_join n Gs with
+    | None => None
+    | Some G' => Some (None :: None :: G')
+    end.
+Proof.
+  intros n Gs.
+  apply partial_fold_left.distr with (mulA := fun x => None :: None :: x)
+                                     (mulB := fun x => None :: None :: x).
+  simpl.
+  intros.
+  repeat break_match; congruence.
+Qed.
+
+Lemma big_join_map_cons_None :
+  forall n Gs,
+    big_join (S n) (map (fun x => None :: x) Gs) =
+    match big_join n Gs with
+    | None => None
+    | Some G' => Some (None :: G')
+    end.
+Proof.
+  intros n Gs.
+  apply partial_fold_left.distr with (mulA := fun x => None :: x) (mulB := fun x => None :: x).
+  reflexivity.
+Qed.
+
+Lemma join_one_Some_inv :
+  forall a b o,
+    join_one (Some a) b = Some o ->
+    o = Some a.
+Proof.
+  unfold join_one.
+  intros.
+  destruct b; congruence.
+Qed.
+
+Lemma join_project1 :
+  forall G1 G2 G,
+    join G1 G2 = Some G ->
+    project None G1 G = G1.
+Proof.
+  unfold join.
+  intros G1 G2 G J.
+  eapply partial_zip_project; [|now apply J].
+  apply join_one_Some_inv.
+Qed.
+
+Lemma join_project2 :
+  forall G1 G2 G,
+    join G1 G2 = Some G ->
+    project None G2 G = G2.
+Proof.
+  intros G1 G2 G J.
+  rewrite join_comm in J.
+  eauto using join_project1.
+Qed.
+
+Lemma empty_length :
+  forall n,
+    length (empty n) = n.
+Proof.
+  induction n; simpl; auto.
+Qed.
+
+Lemma big_join_length_acc :
+  forall Gs n G',
+    big_join n Gs = Some G' ->
+    length G' = n.
+Proof.
+  induction Gs; intros n G' BJ.
+  - cbn in *. invc BJ.
+    auto using empty_length.
+  - rewrite big_join_unroll in BJ.
+    destruct big_join eqn:BJ2; [|discriminate].
+    rename BJ into J.
+    rename BJ2 into BJ.
+    erewrite join_length2 by eauto.
+    eauto.
+Qed.
+
+Lemma big_join_length :
+  forall Gs n G' G1 x,
+    big_join n Gs = Some G' ->
+    nth_error Gs x = Some G1 ->
+    length G1 = n.
+Proof.
+  induction Gs; intros n G' G1 x BJ NE.
+  - destruct x; discriminate.
+  - rewrite big_join_unroll in BJ.
+    destruct big_join eqn:BJ2; [|discriminate].
+    rename BJ into J.
+    rename BJ2 into BJ.
+    destruct x; cbn in NE.
+    + invc NE.
+      erewrite <- join_length1 by eauto.
+      erewrite join_length2 by eauto.
+      eauto using big_join_length_acc.
+    + eapply IHGs; eauto.
+Qed.
+
+Lemma big_join_project :
+  forall Gs G1 G2 G G' n,
+    join G1 G2 = Some G ->
+    big_join n Gs = Some G' ->
+    Forall2 (fun Γ oty => oty = None -> is_empty Γ) Gs G ->
+    exists G1' G2',
+      big_join n (project (empty n) G1 Gs) = Some G1' /\
+      big_join n (project (empty n) G2 Gs) = Some G2' /\
+      join G1' G2' = Some G'.
+Proof.
+  induction Gs; intros G1 G2 G G' n J BJ F.
+  - cbn in BJ. invc BJ.
+    cbn.
+    do 2 eexists.
+    split; [|split]; eauto.
+    now rewrite join_empty_l' by auto using empty_length.
+  - rewrite big_join_unroll in BJ.
+    destruct big_join eqn:BJ2; [|discriminate].
+    rename BJ into J'.
+    rename BJ2 into BJ.
+    invc F.
+    destruct G1, G2; try solve [cbn in J; discriminate].
+    rewrite join_unroll in J.
+    destruct join_one eqn:JO; [|discriminate].
+    destruct join eqn:J12; [|discriminate].
+    invc J.
+
+    eapply IHGs with (G1 := G1) in BJ; eauto.
+    destruct BJ as (G1' & G2' & BJ1' & BJ2' & J).
+    assert (length G1' = n) as LG1' by eauto using big_join_length_acc.
+    assert (length G2' = n) as LG2' by eauto using big_join_length_acc.
+
+    cbn [project].
+    destruct o, o0; try solve [cbn in *; discriminate];
+      rewrite !big_join_unroll, BJ1', BJ2';
+      rewrite !join_empty_l' by auto.
+    + pose proof join_assoc G2' a G1' as JA.
+      rewrite join_comm in JA.
+      rewrite J, J' in JA. symmetry in JA.
+      destruct (join a G1') eqn:JA'; [|discriminate].
+      setoid_rewrite join_comm.
+      eauto.
+    + pose proof join_assoc G1' a G2' as JA.
+      rewrite J, J' in JA. symmetry in JA.
+      destruct (join a G2') eqn:JA'; [|discriminate].
+      eauto.
+    + invc JO.
+      rewrite is_empty_equal_empty with (l := a) in J' by auto.
+      rewrite join_empty_l' in J'
+        by (erewrite <- join_length2 by eauto;
+            erewrite join_length1 by eauto;
+            now rewrite empty_length).
+      invc J'.
+      eauto.
+Qed.
 
 Ltac break_join :=
  match goal with
@@ -372,10 +607,196 @@ Ltac break_join :=
    destruct H as [? ?]; subst
  end.
 
+Lemma is_singleton_cons :
+  forall ty G,
+    is_empty G ->
+    is_singleton 0 ty (Some ty :: G).
+Proof. simpl. auto. Qed.
+Hint Resolve is_singleton_cons.
+
+Lemma is_singleton_skip :
+  forall ty G n,
+    is_singleton n ty G ->
+    is_singleton (S n) ty (None :: G).
+Proof. auto. Qed.
+Hint Resolve is_singleton_skip.
+
+Lemma big_join_is_empty :
+  forall n Gs G',
+    Forall is_empty Gs ->
+    big_join n Gs = Some G' ->
+    is_empty G'.
+Proof.
+  unfold big_join.
+  intros n Gs G' F BJ.
+  eapply partial_fold_left.ind_Some with (P := is_empty); try apply BJ; auto.
+  clear.
+  intros a b b' A B J.
+  apply is_empty_equal_empty in A.
+  apply is_empty_equal_empty in B.
+  pose proof join_length1 _ _ J as L1.
+  pose proof join_length2 _ _ J as L2.
+  rewrite <- L1, <- L2 in *. clear L1 L2.
+  subst a b.
+  rewrite join_empty_l' in J.
+  - invc J. auto.
+  - now rewrite empty_length.
+Qed.
+
+Lemma big_join_is_singleton :
+  forall x ty Gs rho G G1 G',
+    is_singleton x ty G ->
+    Forall3 has_opt_type Gs rho G ->
+    nth_error Gs x = Some G1 ->
+    big_join (length G1) Gs = Some G' ->
+    G' = G1.
+Proof.
+  intros x ty Gs rho G G1 G' IS F NE.
+  revert ty G IS Gs rho G1 G' F NE.
+  induction x; cbn in *; intros ty G IS Gs rho G1 G' F NE BJ.
+  - destruct Gs; [discriminate|].
+    invc NE.
+    rewrite big_join_unroll in BJ.
+    destruct big_join eqn:BJ2; [|discriminate].
+    rename BJ into J.
+    rename BJ2 into BJ.
+    destruct G; cbn in IS; [now intuition|].
+    destruct o; [|now intuition].
+    destruct IS as [? IE]; subst.
+    invc F.
+    apply has_opt_type_Some in H3.
+    apply has_opt_type_empty in H5; [|assumption].
+    apply big_join_is_empty in BJ; [|assumption].
+    apply is_empty_equal_empty in BJ.
+    pose proof join_length2 _ _ J as L.
+    rewrite <- L in *.
+    subst l.
+    erewrite join_length1 in J by eassumption.
+    rewrite join_empty_r in J.
+    congruence.
+  - destruct Gs; [discriminate|].
+    invc F.
+    rewrite big_join_unroll in BJ.
+    destruct big_join eqn:BJ2; [|discriminate].
+    rename BJ into J.
+    rename BJ2 into BJ.
+    cbn in IS.
+    destruct c; [now intuition|].
+    cbn in H1.
+    apply is_empty_equal_empty in H1.
+    erewrite <- join_length1 in H1 by eauto. subst l.
+    erewrite join_length2 in J by eauto.
+    rewrite join_empty_l in J.
+    invc J.
+    eauto.
+Qed.
+
+Lemma is_singleton_app :
+  forall n x ty G,
+    is_singleton x ty G ->
+    is_singleton (x + n) ty (empty n ++ G).
+Proof.
+  intros n x ty G IS.
+  rewrite plus_comm.
+  induction n; auto.
+Qed.
+
+Lemma is_singleton_not_nil :
+  forall x ty G,
+    is_singleton x ty G ->
+    G <> [].
+Proof.
+  intros x ty G IS.
+  apply is_singleton_nth_error1 in IS.
+  intro C.
+  subst.
+  destruct x; discriminate.
+Qed.
+
+Lemma is_empty_app :
+  forall G G',
+    is_empty G ->
+    is_empty G' ->
+    is_empty (G ++ G').
+Proof.
+  induction G; cbn; intros G' IE IE'.
+  - auto.
+  - destruct a; [now intuition|].
+    auto.
+Qed.
+
+Lemma is_empty_splice :
+  forall n n' G,
+    is_empty G ->
+    is_empty (splice n (empty n') G).
+Proof.
+  induction n; cbn; intros n' G IE.
+  - auto using is_empty_app.
+  - destruct G.
+    + now auto.
+    + cbn in *.
+      destruct o; [now intuition|].
+      auto.
+Qed.
+
+Lemma if_pull_f :
+  forall A B (f : A -> B) (b : bool) a1 a2,
+    (if b then f a1 else f a2) = f (if b then a1 else a2).
+Proof.
+  destruct b; auto.
+Qed.
+
+Lemma is_singleton_splice :
+  forall n n' x ty G,
+    is_singleton x ty G ->
+    is_singleton (if x <? n then x else x + n') ty (splice n (empty n') G).
+Proof.
+  induction n; intros n' x ty G IS; simpl splice.
+  - destruct (Nat.ltb_spec0 x 0); [omega|].
+    auto using is_singleton_app.
+  - destruct G eqn:EQG; [now exfalso; eapply is_singleton_not_nil; eauto|].
+    destruct x.
+    + simpl in *. destruct o; intuition. auto using is_empty_splice.
+    + simpl plus.
+      rewrite if_pull_f.
+      simpl is_singleton in *.
+      destruct o; [now auto|].
+      change (S x <? S n) with (x <? n).
+      now auto.
+Qed.
+
+Lemma join_app :
+  forall G1 G2 G G1' G2' G',
+    join G1 G2 = Some G ->
+    join G1' G2' = Some G' ->
+    join (G1 ++ G1') (G2 ++ G2') = Some (G ++ G').
+Proof.
+  apply partial_zip.app.
+Qed.
+
+Lemma join_splice :
+  forall n n' G1 G2 G,
+    join G1 G2 = Some G ->
+    join (splice n (empty n') G1) (splice n (empty n') G2) = Some (splice n (empty n') G).
+Proof.
+  intros.
+  apply partial_zip.splice;
+    auto using join_empty_l', empty_length.
+Qed.
+
+Lemma Forall3_has_opt_type_Forall2_None_is_empty :
+  forall Gs rho G,
+    Forall3 has_opt_type Gs rho G ->
+    Forall2 (fun Γ oty => oty = None -> is_empty Γ) Gs G.
+Proof.
+  induction 1; constructor; auto.
+  now intros ?; subst c.
+Qed.
+
 Module has_type.
   Inductive t : list (option type.t) -> expr.t -> type.t -> Prop :=
   | var : forall G x ty,
-      singleton x ty G ->
+      is_singleton x ty G ->
       t G (expr.var x) ty
   | abs : forall G e ty1 ty2 ,
       t (Some ty1 :: G) e ty2 ->
@@ -405,7 +826,7 @@ Module has_type.
   | snd : forall G e ty1 ty2,
       t G e (type.uchoose ty1 ty2) ->
       t G (expr.snd e) ty2
-  | inl : forall G e ty1 ty2,
+ | inl : forall G e ty1 ty2,
       t G e ty1 ->
       t G (expr.inl e) (type.ichoose ty1 ty2)
   | inr : forall G e ty1 ty2,
@@ -435,116 +856,230 @@ Module has_type.
     end.
   Arguments has_opt_type _ _ _ : simpl nomatch.
 
-  Lemma big_join_singleton :
-    forall x ty Gs rho G G1,
-      singleton x ty G ->
-      Forall3 has_opt_type Gs rho G ->
-      nth_error Gs x = Some G1 ->
-      big_join (empty (length G1)) Gs = Some G1.
-  Admitted.
-
-  Lemma big_join_length :
-    forall acc Gs G' G1 x,
-      big_join acc Gs = Some G' ->
-      nth_error Gs x = Some G1 ->
-      length G1 = length G'.
-  Admitted.
-
-  Lemma singleton_cons :
-    forall ty G,
-      is_empty G ->
-      singleton 0 ty (Some ty :: G).
+  Lemma has_opt_type_None :
+    forall n e,
+      has_opt_type (empty n) e None.
   Proof.
-    intros.
+    unfold has_opt_type.
+    auto using is_empty_empty.
+  Qed.
+  Hint Resolve has_opt_type_None.
+
+  Lemma has_opt_type_None_skip :
+    forall G e,
+      has_opt_type G e None ->
+      has_opt_type (None :: G) e None.
+  Proof.
+    unfold has_opt_type.
+    auto.
+  Qed.
+  Hint Resolve has_opt_type_None_skip.
+
+  Lemma has_opt_type_Some :
+    forall G e ty,
+      has_opt_type G e (Some ty) ->
+      has_type.t G e ty.
+  Proof.
+    intros G e ty HT.
+    now unfold has_opt_type in HT.
+  Qed.
+
+  Lemma has_opt_type_Some_intro :
+    forall G e ty,
+      t G e ty ->
+      has_opt_type G e (Some ty).
+  Proof.
     simpl.
     auto.
   Qed.
-  Hint Resolve singleton_cons.
+  Hint Resolve has_opt_type_Some_intro.
 
-  Lemma big_join_app :
-    forall G1 G2 Gs G',
-      big_join G2 Gs = Some G' ->
-      big_join (G1 ++ G2) (map (fun G => empty (length G1) ++ G) Gs) = Some (G1 ++ G').
-  Admitted.
-
-  Lemma big_join_cons :
-    forall ty acc Gs G',
-      big_join acc Gs = Some G' ->
-      big_join (Some ty :: acc) (map (fun G => None :: G) Gs) = Some (Some ty :: G').
+  Lemma has_opt_type_empty :
+    forall Gs rho G,
+      is_empty G ->
+      Forall3 has_opt_type Gs rho G ->
+      Forall is_empty Gs.
   Proof.
-    intros.
-    now apply big_join_app with (G1 := [Some ty]).
+    intros Gs rho G E F.
+    induction F.
+    + constructor.
+    + simpl in E. destruct c; [now intuition|now auto].
   Qed.
-
-
-  Fixpoint splice A n (l' l : list A) :=
-    match n with
-    | 0 => l' ++ l
-    | S n =>
-      match l with
-      | [] => l' (* bogus *)
-      | x :: l => x :: splice n l' l
-      end
-    end.
 
   Lemma shift :
     forall G e ty,
       t G e ty ->
-      forall n G',
-        t (splice n G' G) (expr.shift n (length G') e) ty.
-  Admitted.
+      forall n n',
+        t (splice n (empty n') G) (expr.shift n n' e) ty.
+  Proof.
+    induction 1; simpl expr.shift; intros n n';
+      try solve [econstructor; eauto using join_splice].
+    - constructor. auto using is_singleton_splice.
+    - constructor. apply IHt with (n := S n).
+    - econstructor; [|now eauto|now apply IHt2 with (n := S (S n))].
+      now eauto using join_splice.
+    - econstructor; [|now eauto| apply IHt2 with (n := S n)|apply IHt3 with (n := S n)].
+      now eauto using join_splice.
+    - constructor.
+      now apply is_empty_splice.
+  Qed.
 
   Lemma shift' :
-    forall G e ty G',
+    forall G e ty n,
       t G e ty ->
-      t (G' ++ G) (expr.shift 0 (List.length G') e) ty.
+      t (empty n ++ G) (expr.shift 0 n e) ty.
   Proof.
     intros.
-    now apply shift with (n := 0) (G' := G').
+    now apply shift with (n := 0) (n' := n).
   Qed.
 
   Lemma shift_cons :
-    forall G e ty ty0,
+    forall G e ty,
       t G e ty ->
-      t (ty0 :: G) (expr.shift 0 1 e) ty.
+      t (None :: G) (expr.shift 0 1 e) ty.
   Proof.
     intros.
-    now apply shift' with (G' := [ty0]).
+    now apply shift' with (n := 1).
   Qed.
+
+  Lemma shift_cons_opt_None :
+    forall G e ty,
+      has_opt_type G e ty ->
+      has_opt_type (None :: G) (expr.shift 0 1 e) ty.
+  Proof.
+    unfold has_opt_type.
+    intros G e [ty|] H; [|now idtac].
+    now apply shift_cons.
+  Qed.
+
+  Lemma shift_cons_opt_None_skip :
+    forall n G e ty,
+      has_opt_type G (expr.shift 0 n e) ty ->
+      has_opt_type (None :: G) (expr.shift 0 (S n) e) ty.
+  Proof.
+    intros n G e ty H.
+    rewrite <- expr.shift_merge with (d2 := 1).
+    now apply shift_cons_opt_None.
+  Qed.
+
+  Let FHO := Forall3_has_opt_type_Forall2_None_is_empty.
 
   Lemma subst :
     forall G e ty,
       has_type.t G e ty ->
-      forall G' Gs rho,
+      forall G' Gs rho n,
         Forall3 has_opt_type Gs rho G ->
-        big_join (empty (List.length G')) Gs = Some G' ->
+        big_join n Gs = Some G' ->
+        n = List.length G' ->
         has_type.t G' (expr.subst rho e) ty.
   Proof.
-    induction 1; intros G' Gs rho F J; cbn [expr.subst].
+    induction 1; intros G' Gs rho n F J EN; cbn [expr.subst]; eauto.
     - simpl expr.subst.
-      pose proof singleton_nth_error1 _ _ _ H as NEty.
+      pose proof is_singleton_nth_error1 _ _ _ H as NEty.
       destruct (Forall3_nth_error3 _ F NEty) as [G1 [e [NEG1 [NEe HT]]]].
       unfold expr.t in *.
-      unfold has_opt_type in HT.
+      apply has_opt_type_Some in HT.
       rewrite NEe.
-      erewrite <- big_join_length in J by eauto.
-      erewrite big_join_singleton in J by eauto.
+      erewrite <- big_join_length with (n := _) in J by eauto.
+      eapply big_join_is_singleton in J; eauto.
       congruence.
     - constructor.
-      apply IHt with (Gs := (Some ty1 :: repeat None (length G')) :: map (fun G => None :: G) Gs).
-      constructor.
-      + now simpl; auto.
-      + apply Forall3_map1, Forall3_map2.
-        eapply Forall3_impl; [|eassumption].
-        clear.
-        unfold has_opt_type.
-        intros G e [ty|] H.
-        now apply shift_cons.
-        now simpl.
-      + cbn[big_join].
-        rewrite join_empty_l' by (now simpl; rewrite repeat_length).
-        now apply big_join_cons.
-  Admitted.
+      apply IHt with (n := S n)
+                     (Gs := (Some ty1 :: empty (length G')) :: map (fun G => None :: G) Gs).
+      + constructor.
+        now simpl; auto.
+        eauto using Forall3_map1, Forall3_map2, Forall3_impl, shift_cons_opt_None.
+      + now rewrite big_join_unroll, big_join_map_cons_None, J, join_unroll, join_empty_l.
+      + simpl. congruence.
+    - pose proof big_join_project _ _ _ H J (FHO F) as (G1' & G2' & J1' & J2' & J').
+      econstructor; [| eapply IHt1 | eapply IHt2 ]; subst;
+        try solve [eauto using join_length1, join_length2].
+      now erewrite <- join_project1 by eauto; auto.
+      now erewrite <- join_project2 by eauto; auto.
+    - pose proof big_join_project _ _ _ H J (FHO F) as (G1' & G2' & J1' & J2' & J').
+      econstructor; [| eapply IHt1| eapply IHt2]; subst;
+        try solve [eauto using join_length1, join_length2].
+      now erewrite <- join_project1 by eauto; auto.
+      now erewrite <- join_project2 by eauto; auto.
+    - pose proof big_join_project _ _ _ H J (FHO F) as (G1' & G2' & J1' & J2' & J').
+      assert (n = length G2') by (subst; eauto using join_length2, eq_sym).
+      econstructor; [| eapply IHt1|
+                     eapply IHt2 with (n := S (S n))
+                                      (Gs := (Some ty2 :: empty (S n)) ::
+                                             (None :: Some ty1 :: empty n) ::
+                                             (map (fun G => None :: None :: G)
+                                                  (project (empty n) G2 Gs)))];
+      try solve [subst; eauto using join_length1, join_length2].
+      + now erewrite <- join_project1 by eauto; auto.
+      + constructor; [now simpl; auto |].
+        constructor; [now simpl; auto |].
+
+        erewrite <- join_project2 with (G2 := G2) at 2 by eauto.
+        eauto 10 using Forall3_map1, Forall3_map2, Forall3_project, Forall3_impl,
+                       shift_cons_opt_None_skip, shift_cons_opt_None.
+      + do 2 rewrite big_join_unroll.
+        rewrite big_join_map_cons_None2, J2'.
+        do 2 rewrite join_unroll.
+        cbn[join_one].
+        rewrite join_empty_l' by congruence.
+        rewrite join_unroll.
+        cbn[join_one].
+        now rewrite join_empty_l' by (cbn; congruence).
+      + cbn. congruence.
+    - pose proof big_join_project _ _ _ H J (FHO F) as (G1' & G2' & J1' & J2' & J').
+      econstructor; [now eauto| | | ].
+      + eapply IHt1; [| now eauto | now subst; eauto using join_length1].
+        now erewrite <- join_project1 by eauto; auto.
+      + apply IHt2 with (n := S n) (Gs := (Some ty1 :: empty n) ::
+                                          map (fun G => None :: G) (project (empty n) G2 Gs));
+          [| |now subst; simpl; eauto using join_length2].
+        constructor; [now auto|].
+        apply Forall3_map1.
+        apply Forall3_map2.
+        erewrite <- join_project2 by eauto.
+        apply Forall3_project.
+        now auto using shift_cons_opt_None.
+        eapply Forall3_impl. 2: eassumption.
+        now auto using shift_cons_opt_None.
+
+        rewrite big_join_unroll.
+        rewrite big_join_map_cons_None.
+        rewrite J2'.
+        rewrite join_unroll.
+        cbn[join_one].
+        now rewrite join_empty_l' by (subst; eauto using join_length2, eq_sym).
+      + apply IHt3 with (n := S n) (Gs := (Some ty2 :: empty n) ::
+                                          map (fun G => None :: G) (project (empty n) G2 Gs));
+          [| |now subst; simpl; eauto using join_length2].
+        constructor; [now auto|].
+        apply Forall3_map1.
+        apply Forall3_map2.
+        erewrite <- join_project2 by eauto.
+        apply Forall3_project.
+        now auto using shift_cons_opt_None.
+        eapply Forall3_impl. 2: eassumption.
+        now auto using shift_cons_opt_None.
+
+        rewrite big_join_unroll.
+        rewrite big_join_map_cons_None.
+        rewrite J2'.
+        rewrite join_unroll.
+        cbn[join_one].
+        now rewrite join_empty_l' by (subst; eauto using join_length2, eq_sym).
+    - econstructor.
+      eapply big_join_is_empty; [|now eauto].
+      now eauto using has_opt_type_empty.
+    - pose proof big_join_project _ _ _ H J (FHO F) as (G1' & G2' & J1' & J2' & J').
+      econstructor; [now eauto| |].
+      + eapply IHt1; [|now eauto|].
+        erewrite <- join_project1 by eauto.
+        apply Forall3_project; auto.
+        subst. eauto using join_length1.
+      + eapply IHt2; [|now eauto|].
+        erewrite <- join_project2 by eauto.
+        apply Forall3_project; auto.
+        subst. eauto using join_length2.
+  Qed.
 End has_type.
 
 Module value.
